More examples

Phi_Examples/PhiEx_BiTree.thy
@@ -57,7 +57,55 @@ declare [[\<phi>trace_reasoning = 0]]
        and Functional_Transformation_Functor
 
 
+term Map.empty
+term \<open>()\<close>
 
+primrec lookup_tree :: \<open>('k \<times> 'v) tree \<Rightarrow> 'k \<rightharpoonup> 'v\<close>
+  where \<open>lookup_tree \<langle>\<rangle> = Map.empty\<close>
+      | \<open>lookup_tree \<langle>L, x, R\<rangle> = (lookup_tree L ++ lookup_tree R)(fst x \<mapsto> snd x) \<close>
+
+lemma dom_lookup_tree[iff]:
+  \<open> dom (lookup_tree tree) = fst ` set_tree tree \<close>
+  by (induct tree; auto_sledgehammer)
+
+primrec tree_domain_distinct :: \<open>('k \<times> 'v) tree \<Rightarrow> bool\<close>
+  where \<open>tree_domain_distinct \<langle>\<rangle> = True \<close>
+      | \<open>tree_domain_distinct \<langle>L, x, R\<rangle> = (fst ` set_tree L \<inter> fst ` set_tree R = {} \<and>
+                                           fst x \<notin> fst ` set_tree L \<and> fst x \<notin> fst ` set_tree R \<and>
+                                           tree_domain_distinct L \<and> tree_domain_distinct R)\<close>
+
+
+
+
+lemma lookup_tree_eq_empty:
+  \<open> lookup_tree tree = Map.empty \<longleftrightarrow> tree = \<langle>\<rangle> \<close>
+  by (induct tree; auto_sledgehammer)
+
+lemma tree_domain_distinct_map[iff]:
+  \<open>tree_domain_distinct (Tree.tree.map_tree (\<lambda>(k, v). (k, f k v)) tree) \<longleftrightarrow> tree_domain_distinct tree\<close>
+  by (induct tree; auto_sledgehammer)
+
+lemma lookup_tree_by_set_distinct:
+  \<open> (k, v) \<in> Tree.tree.set_tree tree
+\<Longrightarrow> tree_domain_distinct tree
+\<Longrightarrow> lookup_tree tree k = Some v \<close>
+  by (induct tree; auto_sledgehammer)
+
+lemma rel_tree_domain_eq:
+  \<open> rel_tree (\<lambda>a b. fst a = fst b) x y
+\<Longrightarrow> fst ` set_tree x = fst ` set_tree y \<close>
+  by (induct x arbitrary: y; auto simp: set_eq_iff rel_tree_Node1; auto_sledgehammer)
+
+lemma rel_tree_domain_distinct:
+  \<open> rel_tree (\<lambda>a b. fst a = fst b) x y
+\<Longrightarrow> tree_domain_distinct x \<longleftrightarrow> tree_domain_distinct y \<close>
+  by (induct x arbitrary: y; auto simp: set_eq_iff rel_tree_Node1; auto_sledgehammer)
+
+lemma rel_map_lookup_by_rel_tree:
+  \<open> rel_tree (\<lambda>a b. fst a = fst b \<and> r (snd a) (snd b)) x y
+\<Longrightarrow> tree_domain_distinct x
+\<Longrightarrow> rel_map r (lookup_tree x) (lookup_tree y) \<close>
+  by (induct x arbitrary: y; auto simp: set_eq_iff rel_fun_def rel_tree_Node1 split: option.split; auto_sledgehammer)
 
 (*
 primrec sorted_tree :: "('a \<Rightarrow> 'k::ord) => 'a tree => bool"
@@ -73,13 +121,121 @@ term cmp
 term lookup
 term map_of
 
+lemma AList_Upd_map_of_is_Map_map_of[iff]:
+  \<open>map_of l = Map.map_of l\<close>
+  by (induct l; auto)
+(*
+lemma dom_lookup_tree_map[iff]:
+  \<open> dom (lookup_tree (map_tree (\<lambda>(k,v). (k, f k v)) tree)) = dom (lookup_tree tree) \<close>
+  by (induct tree; auto_sledgehammer)*)
 
-\<phi>type_def Lookup_Tree :: \<open>logaddr \<Rightarrow> TY \<Rightarrow> (VAL, 'k::linorder) \<phi> \<Rightarrow> (VAL, 'v) \<phi> \<Rightarrow> (fiction, 'k \<rightharpoonup> 'v) \<phi>\<close>
-  where \<open>f \<Ztypecolon> Lookup_Tree addr TY K V \<equiv> tree \<Ztypecolon> BiTree addr TY \<lbrace> k: K, v: V \<rbrace> \<s>\<u>\<b>\<j> tree. f = lookup tree\<close>
+
+
+
+lemma
+  \<open> P (if C then x else y) \<longleftrightarrow> (C \<longrightarrow> P x) \<and> (\<not> C \<longrightarrow> P y)\<close>
   
 
 
 
+
+
+lemma Object_Equive_of_Lookup_Tree:
+  \<open> fst ` Tree.tree.set_tree xa = dom y \<Longrightarrow>
+     tree_domain_distinct xa \<Longrightarrow>
+    y = lookup_tree (Tree.tree.map_tree (\<lambda>(k, _). (k, the (y k))) xa) \<close>
+  apply (induct xa arbitrary: y, auto_sledgehammer,
+         auto simp: fun_eq_iff set_eq_iff map_add_def image_Un Ball_def split: option.split if_split)
+  apply (metis domIff insertI1 option.exhaust_sel)
+  subgoal premises prems for xa1 a xa2 y x
+    apply (cases \<open>x \<in> fst ` set_tree xa1\<close>)
+    subgoal premises prems2 proof -
+      have t2: \<open>Tree.tree.map_tree (\<lambda>(k, _). (k, the ((y |` (fst ` set_tree xa1)) k))) xa1 =
+                Tree.tree.map_tree (\<lambda>(k, _). (k, the (y k))) xa1\<close>
+        by (rule tree.map_cong0, auto_sledgehammer)
+      have \<open>y x = (y |` (fst ` set_tree xa1)) x\<close>
+        unfolding restrict_map_def
+        by auto_sledgehammer
+      also have  \<open>\<dots> = lookup_tree (Tree.tree.map_tree (\<lambda>(k, _). (k, the ((y |` (fst ` set_tree xa1)) k))) xa1) x\<close>
+        by (rule prems(1)[THEN spec]; auto_sledgehammer)
+      finally show ?thesis by auto_sledgehammer
+    qed by auto_sledgehammer
+  apply auto_sledgehammer
+
+  subgoal premises prems for xa1 a xa2 y x x2
+    apply (cases \<open>x \<in> dom (lookup_tree xa2)\<close>)
+    subgoal premises prems2 proof -
+      have t2: \<open>Tree.tree.map_tree (\<lambda>(k, _). (k, the ((y |` (fst ` set_tree xa2)) k))) xa2 =
+                Tree.tree.map_tree (\<lambda>(k, _). (k, the (y k))) xa2\<close>
+        by (rule tree.map_cong0, auto_sledgehammer)
+      have \<open>y x = (y |` (fst ` set_tree xa2)) x\<close>
+        unfolding restrict_map_def
+        by auto_sledgehammer
+      also have  \<open>\<dots> = lookup_tree (Tree.tree.map_tree (\<lambda>(k, _). (k, the ((y |` (fst ` set_tree xa2)) k))) xa2) x\<close>
+        by (rule prems(2)[THEN spec]; auto_sledgehammer)
+      finally show ?thesis by auto_sledgehammer
+    qed by auto_sledgehammer .
+
+lemma rel_tree_self_map:
+  \<open> \<forall>a \<in> set_tree x. R a (f a)
+\<Longrightarrow> rel_tree R x (map_tree f x) \<close>
+  by (induct x; auto)
+
+
+declare rel_fun_eq[iff]
+
+
+
+
+
+
+
+
+
+
+
+  
+\<phi>type_def Lookup_Tree :: \<open>logaddr \<Rightarrow> TY \<Rightarrow> (VAL, 'k::linorder) \<phi> \<Rightarrow> (VAL, 'v) \<phi> \<Rightarrow> (fiction, 'k \<rightharpoonup> 'v) \<phi>\<close>
+  where \<open>f \<Ztypecolon> Lookup_Tree addr TY K V \<equiv> tree \<Ztypecolon> BiTree addr TY \<lbrace> k: K, v: V \<rbrace>
+                                       \<s>\<u>\<b>\<j> tree. f = lookup_tree tree \<and> tree_domain_distinct tree\<close>
+  deriving \<open> Abstract_Domain\<^sub>L K P\<^sub>K
+         \<Longrightarrow> Abstract_Domain V P\<^sub>V
+         \<Longrightarrow> Abstract_Domain (Lookup_Tree addr TY K V) (\<lambda>f. \<forall>x. x \<in> dom f \<and> P\<^sub>K x \<longrightarrow> P\<^sub>V (the (f x))) \<close>
+            (tactic: clarsimp, subgoal' for tree x y \<open>induct tree arbitrary: x\<close>)
+       and \<open>Identity_Elements\<^sub>E (Lookup_Tree addr TY K V) (\<lambda>l. addr = 0 \<and> l = Map.empty)\<close> 
+       and \<open>Identity_Elements\<^sub>I (Lookup_Tree addr TY K V) (\<lambda>l. l = Map.empty) (\<lambda>l. addr = 0)\<close>
+       and \<open> Object_Equiv V eq
+         \<Longrightarrow> Object_Equiv (Lookup_Tree addr TY K V) (\<lambda>f g. dom f = dom g \<and> (\<forall>k \<in> dom f. eq (the (f k)) (the (g k))) ) \<close>  
+            (tactic: clarsimp, 
+                     rule exI[where x=\<open>\<lambda>_ g x. map_tree (\<lambda>(k,_). (k, the (g k))) x\<close>],
+                     auto simp: Object_Equive_of_Lookup_Tree)
+       and \<open> \<c>\<o>\<n>\<d>\<i>\<t>\<i>\<o>\<n> TY' = TY \<and> addr' = addr
+         \<Longrightarrow> Transformation_Functor (Lookup_Tree addr TY K) (Lookup_Tree addr' TY' K) T U ran (\<lambda>_. UNIV) rel_map \<close>
+            (tactic: clarsimp, rule exI[where x=\<open>\<lambda>_ _ y. y\<close>])
+       and \<open>Functional_Transformation_Functor (Lookup_Tree addr TY K) (Lookup_Tree addr TY K) T U ran (\<lambda>_. UNIV)
+                                              (\<lambda>_ P f. \<forall>x \<in> dom f. P (the (f x))) (\<lambda>f _ x. map_option f o x) \<close>
+
+
+
+
+
+
+term \<open> \<c>\<o>\<n>\<d>\<i>\<t>\<i>\<o>\<n> TY' = TY \<and> addr' = addr
+              \<Longrightarrow> Transformation_Functor (Lookup_Tree addr TY K) (Lookup_Tree addr' TY' K) T U ran (\<lambda>_. UNIV) rel_map \<close>
+
+term \<open> Object_Equiv V eq
+         \<Longrightarrow> Object_Equiv (Lookup_Tree addr TY K V) (\<lambda>f g. dom f = dom g \<and> (\<forall>k \<in> dom f. eq (the (f k)) (the (g k))) ) \<close>
+
+
+term \<open>Identity_Elements\<^sub>I (Lookup_Tree addr TY K V) (\<lambda>l. l = Map.empty) (\<lambda>l. addr = 0)\<close>
+
+term \<open>Identity_Elements\<^sub>E (Lookup_Tree addr TY K V) (\<lambda>l. addr = 0 \<and> l = Map.empty)\<close>
+
+(* tactic \<open>Simplifier.asm_full_simp_tac (Config.put Simplifier.simp_trace true
+        (Config.put Simplifier.simp_trace_depth_limit 5 \<^context>)) 1 o @{print}\<close> *)
+term \<open> Abstract_Domain\<^sub>L K P\<^sub>K
+         \<Longrightarrow> Abstract_Domain V P\<^sub>V
+         \<Longrightarrow> Abstract_Domain (Lookup_Tree addr TY K V) (\<lambda>f. \<forall>x. x \<in> dom f \<and> P\<^sub>K x \<longrightarrow> P\<^sub>V (the (f x))) \<close>
 
 
 
